broken/Parametricity.v
@@ -3,9 +3,7 @@ Require Import Arith.
 Require Export Compare_dec.
 Require Export Relations.
 
-Hint Resolve t_step rt_step rt_refl: core.
-Hint Unfold transp: core.
-
+(*
 Inductive ty :=
 | Tvar (v:nat)
 | Tarr (a b:ty)
@@ -15,7 +13,7 @@ Inductive term : Set :=
 | Ref : nat -> term
 | Abs : term -> term
 | App : term -> term -> term.
-
+*)
 
 (* Model *)
 
@@ -109,7 +107,7 @@ Lemma val_ok_thin : forall e i j x,
   val_ok e i j ->
   val_ok (map (tlift 1) e) (UM.cons x i) j.
 unfold val_ok; intros.
-assert (exists2 t, nth_error e n = value t & ty0 = tlift 1 t).
+assert (exists2 t, nth_error e n = value t & ty = tlift 1 t).
  clear i j x H.
  revert e H0; induction n; destruct e; simpl; intros; try discriminate.
   injection H0; exists s; auto.
@@ -229,7 +227,7 @@ Lemma val_ok_thin : forall e i j j' x,
   val_ok e i j j' ->
   val_ok (map (tlift 1) e) (RM.cons x i) j j'.
 unfold val_ok; intros.
-assert (exists2 t, nth_error e n = value t & ty0 = tlift 1 t).
+assert (exists2 t, nth_error e n = value t & ty = tlift 1 t).
  clear i j x H.
  revert e H0; induction n; destruct e; simpl; intros; try discriminate.
   injection H0; exists s; auto.
@@ -296,31 +294,494 @@ unfold tsub; trivial.
 Qed.
 
 End RelSemantics.
+<<<<<<< .mine
+
+Module PropEmbedded.
+
+  (* Embedding propositions in D *)
+
+  Parameter Uprop : Prop -> D.
+  Parameter Uprop_inj : forall P Q, Uprop P = Uprop Q -> P = Q.
+
+  Definition Uprop_inv x := exists2 P, P & x = Uprop P.
+  Lemma Uprop_has_inv : forall P, Uprop_inv (Uprop P) = P.
+intros.
+unfold Uprop_inv.
+apply prop_ext.
+split; intros. (* introduce variable capture... *)
+ destruct H.
+ apply Uprop_inj in H0; rewrite H0; trivial.
+
+ exists P; trivial.
+Qed.
+
+(* OK  model is inconsistent *)
+Lemma has_fix : forall F:D->D, exists x, F x = x.
+intros.
+pose (fx :=
+  let dlt := Dlam (fun x => F (Dapp x x)) in
+  Dapp dlt dlt).
+exists fx.
+unfold fx at 2; simpl.
+rewrite Dbeta.
+reflexivity.
+Qed.
+
+Definition Dnot x := Uprop (forall P:Prop, x = Uprop P -> ~P).
+(* Rk: Dnot non monotonic, maps bottom to a valid prop but maps
+   a valid prop to an invalid prop *)
+
+Lemma paradox : False.
+destruct (has_fix Dnot).
+assert (Dnot x = Uprop False).
+ unfold Dnot; apply f_equal; apply prop_ext.
+ split; intros; try contradiction.
+ generalize H0.
+ apply H0.
+ symmetry; assumption.
+assert (Dnot x = Uprop True).
+ rewrite <- H.
+ unfold Dnot at 1; apply f_equal; apply prop_ext.
+ split; intros; trivial.
+ red; intros.
+ rewrite H0 in H2; apply Uprop_inj in H2; rewrite H2; trivial.
+rewrite H0 in H1; apply Uprop_inj in H1.
+rewrite H1; trivial.
+Qed.
+
+  (* Embedding pairs *)
+  Parameter mkPair : D -> D -> D.
+  Parameter Dfst : D -> D.
+  Parameter Dsnd : D -> D.
+  Parameter fst_eq : forall a b, Dfst (mkPair a b) = a.
+  Parameter snd_eq : forall a b, Dsnd (mkPair a b) = b.
+
+  (* Embedding triples *)
+  Definition mkTriple a b c := mkPair a (mkPair b c).
+  Definition Dfst3 t := Dfst t.
+  Definition Dsnd3 t := Dfst (Dsnd t).
+  Definition Dthd3 t := Dsnd (Dsnd t).
+  Lemma fst3_eq : forall a b c, Dfst3 (mkTriple a b c) = a.
+  Proof (fun a b c => fst_eq _ _).
+  Lemma snd3_eq : forall a b c, Dsnd3 (mkTriple a b c) = b.
+  intros; unfold Dsnd3, mkTriple; rewrite snd_eq; rewrite fst_eq; reflexivity.
+  Qed.
+  Lemma thd3_eq : forall a b c, Dthd3 (mkTriple a b c) = c.
+  intros; unfold Dthd3, mkTriple; do 2 rewrite snd_eq; reflexivity.
+  Qed.
+
+  (* Embedding predicates *)
+
+  Definition mkSet (P:D->Prop) : D :=
+    Dlam (fun x => Uprop (P x)).
+
+  Definition El (t x:D) := Uprop_inv (Dapp t x).
+
+  Lemma Set_beta : forall (R:D->Prop) x,
+    El (mkSet R) x = R x.
+unfold El, mkSet; intros.
+rewrite Dbeta.
+apply Uprop_has_inv.
+Qed.
+
+  (* Embedding relations *)
+
+  Definition mkRel (R:D->D->Prop) : D :=
+    Dlam (fun x => Dlam (fun y => Uprop (R x y))).
+
+  Definition Rel (r x y:D) := Uprop_inv (Dapp (Dapp r x) y).
+
+  Lemma Rel_beta : forall (R:D->D->Prop) x y,
+    Rel (mkRel R) x y = R x y.
+unfold Rel, mkRel; intros.
+do 2 rewrite Dbeta.
+apply Uprop_has_inv.
+Qed.
+
+End PropEmbedded.
 
 
-Module Beq.
-Definition t := bool.
-Definition eq := @eq bool.
-Definition eq_equiv : Equivalence eq := eq_equivalence.
-Existing Instance eq_equiv.
-End Beq.
-Module B := VarMap.Make(Beq).
+Module CocSemantics.
+  Import PropEmbedded.
 
-Record fenv := {
-  tenv : list trm;
-  impl : B.map
-}.
 
-Definition tinj e :=
-  Build_fenv e (B.nil false).
+  Definition Dprop := mkSet
+    (fun x => exists P:Prop, x = mkSet(fun y => y = Uprop False /\ P)).
 
-Definition push_var e T :=
-  Build_fenv (T::tenv e) (B.cons false (impl e)).
+  Definition Dprod A F :=
+    mkSet (fun f => forall x, El A x -> El (F x) (Dapp f x)).
 
-Definition push_ivar e T :=
-  Build_fenv (T::tenv e) (B.cons true (impl e)).
 
-Module ICocSemantics.
+  Definition prop : trm := fun _ => Dprop.
+
+  Definition prod (A B:trm) : trm :=
+    fun i => Dprod (A i) (fun x => B (DM.cons x i)).
+
+(* OK  model is inconsistent (models Type:Type)
+  Definition Dkind := mkSet (fun _ => True).
+
+Lemma sysU : El Dkind Dkind.
+unfold Dkind at 1.
+rewrite Set_beta.
+trivial.
+Qed.
+*)
+ 
+Definition val_ok (e:list trm) i :=
+  forall n ty, nth_error e n = value ty ->
+  El (ty (DM.shift (S n) i)) (i n).
+
+Lemma val_ok_cons : forall e i x (ty:trm),
+  val_ok e i ->
+  El (ty i) x ->
+  val_ok (ty::e) (DM.cons x i).
+red; intros.
+destruct n as [|n]; simpl in *.
+ injection H1; clear H1; intros; subst ty0.
+ replace (DM.shift 1 (DM.cons x i)) with i; auto.
+ apply ext; reflexivity.
+
+ change (DM.shift (S (S n)) (DM.cons x i)) with (DM.shift (S n) i).
+ apply H; trivial.
+Qed.
+(*
+Lemma val_ok_thin : forall e i i' x x',
+  val_ok e i i' ->
+  val_ok (map (lift 1) e) (DM.cons x i) (DM.cons x' i').
+unfold val_ok; intros.
+assert (exists2 t, nth_error e n = value t & ty0 = lift 1 t).
+ clear i i' x x' H.
+ revert e H0; induction n; destruct e; simpl; intros; try discriminate.
+  injection H0; exists t; auto.
+
+  specialize IHn with (1:=H0).
+  destruct IHn.
+  exists x; trivial.
+destruct H1.
+rewrite H2.
+unfold lift.
+replace (DM.shift 1 (DM.shift (S n) (DM.cons x i)))
+ with (DM.shift (S n) i); auto.
+replace (RM.shift 1 (RM.cons x i)) with i; auto.
+apply ext; intro.
+reflexivity.
+Qed.
+*)
+
+Definition sjudge (e:list trm) (M T:trm) :=
+  forall i, val_ok e i -> El (T i) (M i).
+
+Lemma ty_ref : forall (e:list trm) n ty,
+  nth_error e n = value ty ->
+  sjudge e (ref n) (lift (S n) ty).
+red; intros.
+apply H0; trivial.
+Qed.
+
+
+Lemma ty_app : forall e u v A B,
+  sjudge e u (prod A B) ->
+  sjudge e v A ->
+  sjudge e (app u v) (sub v B).
+unfold sjudge; intros.
+specialize H with (1:=H1).
+specialize H0 with (1:=H1).
+unfold prod, Dprod in H.
+rewrite Set_beta in H.
+unfold sub, app.
+auto.
+Qed.
+
+Lemma ty_abs : forall e m T U,
+  sjudge (T::e) m U ->
+  sjudge e (abs m) (prod T U).
+unfold sjudge; intros.
+unfold prod, Dprod; rewrite Set_beta.
+intros.
+assert (val_ok (T::e) (DM.cons x i)).
+ apply val_ok_cons; trivial.
+specialize H with (1:=H2).
+unfold abs.
+rewrite Dbeta.
+trivial.
+Qed.
+
+Lemma conv_beta : forall m v, app (abs m) v = sub v m.
+intros.
+apply ext; intro i.
+unfold app, abs, sub.
+rewrite Dbeta.
+trivial.
+Qed.
+
+End CocSemantics.
+
+
+Module CocSetoidSemantics.
+  Import PropEmbedded.
+
+  Definition Dprop := mkRel (fun x y => x=y /\ exists P:Prop, x = Uprop P).
+
+  Definition Dprod A F :=
+    mkRel (fun f f' =>
+      forall x x',
+      Rel A x x' ->
+      Rel (F x x') (Dapp f x) (Dapp f' x')).
+
+  Definition prop : trm := fun _ => Dprop.
+
+  Definition prod (A B:trm) : trm :=
+    fun i => Dprod (A i) (fun x x' => B (DM.cons x i) (DM.cons x' i)).
+
+
+Module CocNaiveRelSemantics.
+  Import PropEmbedded.
+
+  Definition Dprop := mkRel (fun x y => x=y /\ exists P:Prop, x = Uprop P).
+
+  Definition Dprod A F :=
+    mkRel (fun f f' => forall x x', Rel A x x' -> Rel (F x) (Dapp f x) (Dapp f' x')).
+
+  Definition prop : trm := fun _ => Dprop.
+
+  Definition prod (A B:trm) : trm :=
+    fun i => Dprod (A i) (fun x => B (DM.cons x i)).
+
+Definition val_ok (e:list trm) i i' :=
+  forall n ty, nth_error e n = value ty ->
+  Rel (ty (DM.shift (S n) i)) (i n) (i' n).
+
+Lemma val_ok_cons : forall e i i' x x' (ty:trm),
+  val_ok e i i' ->
+  Rel (ty i) x x' ->
+  val_ok (ty::e) (DM.cons x i) (DM.cons x' i').
+red; intros.
+destruct n as [|n]; simpl in *.
+ injection H1; clear H1; intros; subst ty0.
+ replace (DM.shift 1 (DM.cons x i)) with i; auto.
+ apply ext; reflexivity.
+
+ change (DM.shift (S (S n)) (DM.cons x i)) with (DM.shift (S n) i).
+ apply H; trivial.
+Qed.
+
+Definition sjudge (e:list trm) (M M' T:trm) :=
+  forall i i', val_ok e i i' -> Rel (T i) (M i) (M' i').
+
+Lemma ty_ref : forall (e:list trm) n ty,
+  nth_error e n = value ty ->
+  sjudge e (ref n) (ref n) (lift (S n) ty).
+red; intros.
+red in H0.
+unfold lift.
+apply H0; trivial.
+Qed.
+
+Lemma ty_app : forall e u u' v v' A B,
+  sjudge e u u' (prod A B) ->
+  sjudge e v v' A ->
+  sjudge e (app u v) (app u' v') (sub v B).
+unfold sjudge; intros.
+specialize H with (1:=H1).
+specialize H0 with (1:=H1).
+unfold prod, Dprod in H.
+rewrite Rel_beta in H.
+unfold sub, app.
+auto.
+Qed.
+
+Definition is_kind (e:list trm) (T T':trm) :=
+  forall i i', val_ok e i i' -> T i = T' i'.
+
+Lemma ty_abs : forall e m m' T U,
+  sjudge (T::e) m m' U ->
+  sjudge e (abs m) (abs m') (prod T U).
+unfold sjudge; intros.
+unfold prod, Dprod; rewrite Rel_beta.
+intros.
+assert (val_ok (T::e) (DM.cons x i) (DM.cons x' i')).
+ apply val_ok_cons; trivial.
+specialize H with (1:=H2).
+unfold abs.
+do 2 rewrite Dbeta.
+trivial.
+Qed.
+
+Lemma ty_beta : forall e T U m m' v v',
+  sjudge (T::e) m m' U ->
+  sjudge e v v' T ->
+  sjudge e (app (abs m) v) (sub v' m') (sub v U).
+unfold sjudge, app, abs, sub; intros.
+rewrite Dbeta.
+apply H.
+apply val_ok_cons; auto.
+Qed.
+
+Lemma ty_conv : forall e m m' T T',
+  sjudge e m m' T ->
+  is_kind e T T' ->
+  sjudge e m m' T'.
+unfold is_kind, sjudge; intros.
+rewrite <- (H0 i i); auto.
+Abort. (* (val_ok e i i) *)
+
+
+
+Module CocRelSemantics.
+  Import PropEmbedded.
+
+  Definition Dprop := mkRel (fun x y => x=y /\ exists P:Prop, x = Uprop P).
+
+  Definition Dprod A F :=
+    mkRel (fun f f' => forall x x', Rel A x x' -> Rel (F x) (Dapp f x) (Dapp f' x')).
+
+  Definition prop : trm := fun _ => Dprop.
+
+  Definition prod (A B:trm) : trm :=
+    fun i => Dprod (A i) (fun x => B (DM.cons x i)).
+
+  Definition mkObj x := Dlam(fun fobj => Dlam(fun fty => Dapp fobj x)).
+  Definition mkTy r := Dlam(fun fobj => Dlam(fun fty => Dapp fty (mkRel r))).
+
+  Definition Sem_elim fobj fty d := Dapp (Dapp d fobj) fty.
+
+  Definition Ty :=
+    Sem_elim (Dlam(fun _=>mkRel(fun _ _ => False)))
+             (Dlam(fun R => R)).
+
+  Definition Fst :=
+    Sem_elim (Dlam Dfst)
+             (Dlam(fun R => mkTy(fun x x' => exists2 y, Rel R x y & Rel R x' y))).
+
+  Definition Snd :=
+    Sem_elim (Dlam Dsnd)
+             (Dlam(fun R => mkTy(fun y y' => exists2 x, Rel R x y & Rel R x y'))).
+
+  Lemma red_Ty : forall fobj fty r, Sem_elim fobj fty (mkTy r) = Dapp fty (mkRel r).
+intros; unfold Sem_elim, mkTy.
+do 2 rewrite Dbeta; trivial.
+Qed.
+  Lemma red_Obj : forall fobj fty p, Sem_elim fobj fty (mkObj p) = Dapp fobj p.
+intros; unfold Sem_elim, mkObj.
+do 2 rewrite Dbeta; trivial.
+Qed.
+
+  Lemma Ty_simpl : forall r, Ty (mkTy r) = mkRel r.
+intros; unfold Ty.
+rewrite red_Ty.
+rewrite Dbeta; trivial.
+Qed.
+
+  Definition DMcomp (f:D->D) (i:DM.map) : DM.map := fun k => f (i k). 
+
+Definition val_ok (e:list trm) i :=
+  forall n ty, nth_error e n = value ty ->
+  Rel (ty (DM.shift (S n) (DMcomp Ty i))) (Fst (i n)) (Snd (i n)).
+
+Lemma val_ok_cons : forall e i x (ty:trm),
+  val_ok e i ->
+  Rel (ty (DMcomp Ty i)) (Fst x) (Snd x) ->
+  val_ok (ty::e) (DM.cons x i).
+red; intros.
+destruct n as [|n]; simpl in *.
+ injection H1; clear H1; intros; subst ty0.
+ exact H0.
+
+ change (DM.shift (S (S n)) (DMcomp Ty (DM.cons x i))) with (DM.shift (S n) (DMcomp Ty i)).
+ apply H; trivial.
+Qed.
+(*
+Lemma val_ok_thin : forall e i i' x x',
+  val_ok e i i' ->
+  val_ok (map (lift 1) e) (DM.cons x i) (DM.cons x' i').
+unfold val_ok; intros.
+assert (exists2 t, nth_error e n = value t & ty0 = lift 1 t).
+ clear i i' x x' H.
+ revert e H0; induction n; destruct e; simpl; intros; try discriminate.
+  injection H0; exists t; auto.
+
+  specialize IHn with (1:=H0).
+  destruct IHn.
+  exists x; trivial.
+destruct H1.
+rewrite H2.
+unfold lift.
+replace (DM.shift 1 (DM.shift (S n) (DM.cons x i)))
+ with (DM.shift (S n) i); auto.
+replace (RM.shift 1 (RM.cons x i)) with i; auto.
+apply ext; intro.
+reflexivity.
+Qed.
+*)
+
+Definition sjudge (e:list trm) (M M' T:trm) :=
+  forall i, val_ok e i -> Rel (T (DMcomp Ty i)) (M (DMcomp Fst i)) (M' (DMcomp Snd i)).
+
+Lemma ty_ref : forall (e:list trm) n ty,
+  nth_error e n = value ty ->
+  sjudge e (ref n) (ref n) (lift (S n) ty).
+red; intros.
+red in H0.
+unfold lift.
+apply H0; trivial.
+Qed.
+
+Lemma ty_app : forall e u u' v v' A B,
+  sjudge e u u' (prod A B) ->
+  sjudge e v v' A ->
+  sjudge e (app u v) (app u' v') (sub v B).
+unfold sjudge; intros.
+specialize H with (1:=H1).
+specialize H0 with (1:=H1).
+unfold prod, Dprod in H.
+rewrite Rel_beta in H.
+unfold sub, app.
+
+auto.
+Qed.
+
+Definition PER (r:D) := Symmetric (Rel r) /\ Transitive (Rel r).
+
+Definition is_kind (e:list trm) (T T':trm) :=
+  forall i i', val_ok e i i' -> T i = T' i'.
+
+Lemma ty_abs : forall e m m' T U,
+  sjudge (T::e) m m' U ->
+  sjudge e (abs m) (abs m') (prod T U).
+unfold sjudge; intros.
+unfold prod, Dprod; rewrite Rel_beta.
+intros.
+assert (val_ok (T::e) (DM.cons x i) (DM.cons x' i')).
+ apply val_ok_cons; trivial.
+specialize H with (1:=H2).
+unfold abs.
+do 2 rewrite Dbeta.
+trivial.
+Qed.
+
+Lemma ty_beta : forall e T U m m' v v',
+  sjudge (T::e) m m' U ->
+  sjudge e v v' T ->
+  sjudge e (app (abs m) v) (sub v' m') (sub v U).
+unfold sjudge, app, abs, sub; intros.
+rewrite Dbeta.
+apply H.
+apply val_ok_cons; auto.
+Qed.
+
+Lemma ty_conv : forall e m m' T T',
+  sjudge e m m' T ->
+  is_kind e T T' ->
+  sjudge e m m' T'.
+unfold is_kind, sjudge; intros.
+assert (val_ok e i i).
+ admit.
+specialize H0 with (1:=H2).
+rewrite <- H0; auto.
+Qed.
+=======
+
+Module CocSemantics.
 
   Parameter Uprop : Prop -> D.
   Parameter Uprop_inj : forall P Q, Uprop P = Uprop Q -> P = Q.
@@ -404,22 +865,15 @@ rewrite H0 in H1; apply Uprop_inj in H1.
 rewrite H1; trivial.
 Qed.
 *)
-
-(* Additional judgments for fix body *)
-Definition val_ok (e:fenv) i :=
-    forall n ty,
-    nth_error (tenv e) n = value ty ->
-    El (ty (DM.shift (S n) i)) (i n).
-
-Definition val_mono (e:fenv) (i i':DM.map) :=
-  forall n,
-  if impl e n then True
-  else i n = i' n.
+ 
+Definition val_ok (e:list trm) i :=
+  forall n ty, nth_error e n = value ty ->
+  El (ty (DM.shift (S n) i)) (i n).
 
 Lemma val_ok_cons : forall e i x (ty:trm),
   val_ok e i ->
   El (ty i) x ->
-  val_ok (push_var e ty) (DM.cons x i).
+  val_ok (ty::e) (DM.cons x i).
 red; intros.
 destruct n as [|n]; simpl in *.
  injection H1; clear H1; intros; subst ty0.
@@ -428,14 +882,6 @@ destruct n as [|n]; simpl in *.
 
  change (DM.shift (S (S n)) (DM.cons x i)) with (DM.shift (S n) i).
  apply H; trivial.
-Qed.
-
-Lemma val_mono_cons : forall e i i' x (ty:trm),
-  val_mono e i i' ->
-  val_mono (push_var e ty) (DM.cons x i) (DM.cons x i').
-red; intros.
-destruct n as [|n]; simpl in *; auto.
-apply H.
 Qed.
 (*
 Lemma val_ok_thin : forall e i i' x x',
@@ -461,26 +907,14 @@ reflexivity.
 Qed.
 *)
 
-Definition sjudge (e:fenv) (M T:trm) :=
-  (forall i i', val_ok e i -> val_mono e i i' -> El (T i) (M i')) /\
-  (forall i i', val_mono e i i' -> M i = M i').
+Definition sjudge (e:list trm) (M T:trm) :=
+  forall i, val_ok e i -> El (T i) (M i).
 
-Lemma ty_ref : forall e n ty,
-  nth_error (tenv e) n = value ty ->
-  impl e n = false ->
+Lemma ty_ref : forall (e:list trm) n ty,
+  nth_error e n = value ty ->
   sjudge e (ref n) (lift (S n) ty).
-split; intros.
- red in H1,H2.
- specialize H2 with n.
- rewrite H0 in H2.
- apply H1 in H.
- rewrite H2 in H.
- trivial.
-
- unfold ref.
- red in H1.
- specialize H1 with n.
- rewrite H0 in H1; trivial.
+red; intros.
+apply H0; trivial.
 Qed.
 
 
@@ -488,56 +922,27 @@ Lemma ty_app : forall e u v A B,
   sjudge e u (prod A B) ->
   sjudge e v A ->
   sjudge e (app u v) (sub v B).
-split; intros.
- destruct H; destruct H0.
- specialize H with (1:=H1) (2:=H2).
- specialize H0 with (1:=H1) (2:=H2).
- unfold prod, Dprod in H.
- rewrite Set_beta in H.
- unfold sub, app.
- rewrite H4 with (1:=H2).
- auto.
-
- destruct H; destruct H0.
- unfold app.
- rewrite H2 with (1:=H1); rewrite H3 with (1:=H1); trivial.
+unfold sjudge; intros.
+specialize H with (1:=H1).
+specialize H0 with (1:=H1).
+unfold prod, Dprod in H.
+rewrite Set_beta in H.
+unfold sub, app.
+auto.
 Qed.
 
 Lemma ty_abs : forall e m T U,
-  sjudge (push_var e T) m U ->
+  sjudge (T::e) m U ->
   sjudge e (abs m) (prod T U).
-split; intros.
- destruct H.
- unfold prod, Dprod; rewrite Set_beta.
- intros.
- assert (val_mono (push_var e T) (DM.cons x i) (DM.cons x i')).
-  apply val_mono_cons; trivial.
- unfold abs.
- rewrite Dbeta.
- apply H; auto.
- apply val_ok_cons; auto.
-
- unfold abs.
- apply f_equal.
- apply ext; intros.
- destruct H.
- apply H1.
- apply val_mono_cons; auto.
-Qed.
-
-Definition is_kind e (T T':trm) :=
-  forall i i', val_mono e i i' -> T i = T' i'.
-
-Lemma ty_conv : forall ivars e m m' T T',
-  sjudge ivars e m m' T ->
-  is_kind (B.nil false) e T T' ->
-  sjudge ivars e m m' T'.
-unfold is_kind, sjudge; intros.
-assert (val_ok (B.nil false) e i i).
- red; intros.
- admit.
-specialize H0 with (1:=H2).
-rewrite <- H0; auto.
+unfold sjudge; intros.
+unfold prod, Dprod; rewrite Set_beta.
+intros.
+assert (val_ok (T::e) (DM.cons x i)).
+ apply val_ok_cons; trivial.
+specialize H with (1:=H2).
+unfold abs.
+rewrite Dbeta.
+trivial.
 Qed.
 
 Lemma conv_beta : forall m v, app (abs m) v = sub v m.
@@ -635,25 +1040,15 @@ rewrite H0 in H1; apply Uprop_inj in H1.
 rewrite H1; trivial.
 Qed.
 *)
-
-Module Beq.
-Definition t := bool.
-Definition eq := @eq bool.
-Definition eq_equiv : Equivalence eq := eq_equivalence.
-Existing Instance eq_equiv.
-End Beq.
-Module B := VarMap.Make(Beq).
-
  
-Definition val_ok (ivars:B.map) (e:list trm) i i' :=
+Definition val_ok (e:list trm) i i' :=
   forall n ty, nth_error e n = value ty ->
-  ivars n = false ->
   Rel (ty (DM.shift (S n) i)) (i n) (i' n).
 
-Lemma val_ok_cons : forall ivars e i i' x x' (ty:trm),
-  val_ok ivars e i i' ->
+Lemma val_ok_cons : forall e i i' x x' (ty:trm),
+  val_ok e i i' ->
   Rel (ty i) x x' ->
-  val_ok (B.cons false ivars) (ty::e) (DM.cons x i) (DM.cons x' i').
+  val_ok (ty::e) (DM.cons x i) (DM.cons x' i').
 red; intros.
 destruct n as [|n]; simpl in *.
  injection H1; clear H1; intros; subst ty0.
@@ -663,20 +1058,6 @@ destruct n as [|n]; simpl in *.
  change (DM.shift (S (S n)) (DM.cons x i)) with (DM.shift (S n) i).
  apply H; trivial.
 Qed.
-
-
-Lemma val_ok_cons_impl : forall ivars e i i' x x' (ty:trm),
-  val_ok ivars e i i' ->
-  val_ok (B.cons true ivars) (ty::e) (DM.cons x i) (DM.cons x' i').
-red; intros.
-destruct n as [|n]; simpl in *.
- discriminate H1.
-
- change (DM.shift (S (S n)) (DM.cons x i)) with (DM.shift (S n) i).
- apply H; trivial.
-Qed.
-
-
 (*
 Lemma val_ok_thin : forall e i i' x x',
   val_ok e i i' ->
@@ -701,21 +1082,20 @@ reflexivity.
 Qed.
 *)
 
-Definition sjudge ivars (e:list trm) (M M' T:trm) :=
-  forall i i', val_ok ivars e i i' -> Rel (T i) (M i) (M' i').
+Definition sjudge (e:list trm) (M M' T:trm) :=
+  forall i i', val_ok e i i' -> Rel (T i) (M i) (M' i').
 
-Lemma ty_ref : forall ivars (e:list trm) n ty,
-  ivars n = false ->
+Lemma ty_ref : forall (e:list trm) n ty,
   nth_error e n = value ty ->
-  sjudge ivars e (ref n) (ref n) (lift (S n) ty).
+  sjudge e (ref n) (ref n) (lift (S n) ty).
 red; intros.
-apply H1; trivial.
+apply H0; trivial.
 Qed.
 
-Lemma ty_app : forall ivars e u u' v v' A B,
-  sjudge ivars e u u' (prod A B) ->
-  sjudge ivars e v v' A ->
-  sjudge ivars e (app u v) (app u' v') (sub v B).
+Lemma ty_app : forall e u u' v v' A B,
+  sjudge e u u' (prod A B) ->
+  sjudge e v v' A ->
+  sjudge e (app u v) (app u' v') (sub v B).
 unfold sjudge; intros.
 specialize H with (1:=H1).
 specialize H0 with (1:=H1).
@@ -727,43 +1107,41 @@ Qed.
 
 Definition PER (r:D) := Symmetric (Rel r) /\ Transitive (Rel r).
 
-Definition is_kind ivars (e:list trm) (T T':trm) :=
-  forall i i', val_ok ivars e i i' -> T i = T' i'.
+Definition is_kind (e:list trm) (T T':trm) :=
+  forall i i', val_ok e i i' -> T i = T' i'.
 
-Lemma ty_abs : forall ivars b e m m' T U,
-  sjudge (B.cons b ivars) (T::e) m m' U ->
-  sjudge ivars e (abs m) (abs m') (prod T U).
+Lemma ty_abs : forall e m m' T U,
+  sjudge (T::e) m m' U ->
+  sjudge e (abs m) (abs m') (prod T U).
 unfold sjudge; intros.
 unfold prod, Dprod; rewrite Rel_beta.
 intros.
-assert (val_ok (B.cons b ivars) (T::e) (DM.cons x i) (DM.cons x' i')).
- destruct b.
-  apply val_ok_cons_impl; trivial.
-  apply val_ok_cons; trivial.
+assert (val_ok (T::e) (DM.cons x i) (DM.cons x' i')).
+ apply val_ok_cons; trivial.
 specialize H with (1:=H2).
 unfold abs.
 do 2 rewrite Dbeta.
 trivial.
 Qed.
 
-Lemma ty_beta : forall ivars e T U m m' v v',
-  sjudge (B.cons false ivars) (T::e) m m' U ->
-  sjudge ivars e v v' T ->
-  sjudge ivars e (app (abs m) v) (sub v' m') (sub v U).
+Lemma ty_beta : forall e T U m m' v v',
+  sjudge (T::e) m m' U ->
+  sjudge e v v' T ->
+  sjudge e (app (abs m) v) (sub v' m') (sub v U).
 unfold sjudge, app, abs, sub; intros.
 rewrite Dbeta.
 apply H.
 apply val_ok_cons; auto.
 Qed.
 
-Lemma ty_conv : forall ivars e m m' T T',
-  sjudge ivars e m m' T ->
-  is_kind (B.nil false) e T T' ->
-  sjudge ivars e m m' T'.
+Lemma ty_conv : forall e m m' T T',
+  sjudge e m m' T ->
+  is_kind e T T' ->
+  sjudge e m m' T'.
 unfold is_kind, sjudge; intros.
-assert (val_ok (B.nil false) e i i).
- red; intros.
+assert (val_ok e i i).
  admit.
 specialize H0 with (1:=H2).
 rewrite <- H0; auto.
 Qed.
+>>>>>>> .r190
